Rename `eraseMany` to `eraseManyEntries`

src/Std/Data/DHashMap/Internal/Defs.lean
@@ -452,7 +452,7 @@ def insertMany {ρ : Type w} [ForIn Id ρ ((a : α) × β a)] [BEq α] [Hashable
   return r
 
 /-- Internal implementation detail of the hash map -/
-def eraseMany {ρ : Type w} [ForIn Id ρ ((a : α) × β a)] [BEq α] [Hashable α]
+def eraseManyEntries {ρ : Type w} [ForIn Id ρ ((a : α) × β a)] [BEq α] [Hashable α]
     (m : Raw₀ α β) (l : ρ) : { m' : Raw₀ α β // ∀ (P : Raw₀ α β → Prop),
       (∀ {m'' a}, P m'' → P (m''.erase a)) → P m → P m' } := Id.run do
   let mut r : { m' : Raw₀ α β // ∀ (P : Raw₀ α β → Prop),
@@ -492,7 +492,7 @@ def inter [BEq α] [Hashable α] (m₁ m₂ : Raw₀ α β) : Raw₀ α β :=
 
 /-- Internal implementation detail of the hash map -/
 @[inline] def diff [BEq α] [Hashable α] (m₁ m₂ : Raw₀ α β) : Raw₀ α β :=
-  if m₁.1.size ≤ m₂.1.size then m₁.filter (fun k _ => !m₂.contains k) else (eraseMany m₁ m₂.1).1
+  if m₁.1.size ≤ m₂.1.size then m₁.filter (fun k _ => !m₂.contains k) else (eraseManyEntries m₁ m₂.1).1
 
 
 section
